reify/reflect progress

experiments/mst_handleaway/MSTReifyReflect.fst
@@ -6,6 +6,26 @@ open FStar.Tactics.Typeclasses
 open MST
 open MST.Tot
 
+unfold
+let eq_wp wp1 wp2 = wp1 ⊑ wp2 /\ wp2 ⊑ wp1
+
+unfold
+let eq_wp_f (f:'a -> 'b) (wp1:st_wp 'a) (wp2:st_wp 'b) =
+  st_bind_wp _ _ _ wp1 (fun r -> st_return _ _ (f r)) `eq_wp` wp2
+
+let lemma_eq_wp_f #a #b (w:st_wp a) (f:a -> b) :
+  Lemma
+    (ensures (w `eq_wp_f f` (st_bind_wp _ _ _ w (fun x -> st_return _ _ (f x))))) = () (** REFL **)
+
+let rec lemma_theta_bind_pure (m:mheap 'a 'w) (f:'a -> 'b) :
+  Lemma (ensures (theta m `eq_wp_f f` theta (mheap_bind _ _ _ _ m (fun x -> mheap_return _ (f x))))) (decreases m) = admit ()
+
+let lemma_theta_bind_id (m:mheap 'a 'w) :
+  Lemma (eq_wp 
+    (theta (mheap_bind 'a 'a 'w (fun x -> st_return _ 'a x) m (fun x -> mheap_return 'a x)))
+    (theta m)) = 
+  lemma_theta_bind_pure m id
+
 class lang_effect (t:Type) = { [@@@no_method] _empty : unit }
 
 instance lang_effect_int : lang_effect int = { _empty = () }
@@ -74,7 +94,7 @@ instance my_reflectable_arrow
   (wp:(x:c1.t -> st_wp (t2 x))) 
   : my_reflectable (x:c1.t -> mheap (t2 x) (wp x)) = {
   t_tc = lang_repr_arrow c1.t #c1.t_tc t2 #(fun x -> (c2 x).t_tc) wp;
-  s = x:s1 -> STATEwp (c2 (c1.my_reify x)).s (fun p -> wp (c1.my_reify x) (fun (r:t2 (c1.my_reify x)) -> p ((c2 (c1.my_reify x)).my_reflect r)));
+  s = x:s1 -> STATEwp (c2 (c1.my_reify x)).s (fun (p:st_post (c2 (c1.my_reify x)).s) -> wp (c1.my_reify x) (fun (r:t2 (c1.my_reify x)) -> p ((c2 (c1.my_reify x)).my_reflect r)));
   s_tc = lang_effect_arrow s1 #c1.s_tc (fun (x:s1) -> (c2 (c1.my_reify x)).s) #(fun (x:s1) -> (c2 (c1.my_reify x)).s_tc) _;
   my_reflect = (fun (f:(x:c1.t -> mheap (t2 x) (wp x))) ->
     let f' (x:s1) : mheap (c2 (c1.my_reify x)).s (fun p -> wp (c1.my_reify x) (fun (r:t2 (c1.my_reify x)) -> p ((c2 (c1.my_reify x)).my_reflect r))) = begin 
@@ -102,30 +122,52 @@ instance my_reifiable_pair (s1:Type) {| c1:my_reifiable s1 |} (s2:Type) {| c2:my
   my_reify = (fun (x, y) -> (c1.my_reify x, c2.my_reify y));
 }
 
+let helper_reifiable_arrow_wp 
+  (s1:Type)
+  (s2:s1 -> Type) {| c2:(x:s1 -> my_reifiable (s2 x)) |}
+  (wp:(x:s1 -> st_wp (s2 x)))
+  (x' : s1)
+  : st_wp (c2 x').t =
+  (fun (p:(st_post (c2 x').t)) -> wp x' (fun (r:s2 x') -> p ((c2 x').my_reify r)))
+
+let helper_reifiable_arrow
+  (s1:Type)
+  (s2:s1 -> Type) {| c2:(x:s1 -> my_reifiable (s2 x)) |}
+  (wp:(x:s1 -> st_wp (s2 x))) 
+  (f:(x:s1 -> STATEwp (s2 x) (wp x)))
+  (x':s1)
+  : STATEwp (c2 x').t (helper_reifiable_arrow_wp s1 s2 #c2 wp x') =
+  (c2 x').my_reify (f x')
+
+let helper_reifiable_arrow'
+  (t1:Type) {| c1:my_reflectable t1 |}
+  (s2:c1.s -> Type) {| c2:(x:c1.s -> my_reifiable (s2 x)) |}
+  (wp:(x:c1.s -> st_wp (s2 x))) 
+  (f:(x:c1.s -> STATEwp (s2 x) (wp x)))
+  (x:t1)
+  : STATEwp (c2 (c1.my_reflect x)).t (helper_reifiable_arrow_wp c1.s s2 #c2 wp (c1.my_reflect x)) =
+  helper_reifiable_arrow c1.s s2 #c2 wp f (c1.my_reflect x)
+
 instance my_reifiable_arrow 
   (t1:Type) {| c1:my_reflectable t1 |}
   (s2:c1.s -> Type) {| c2:(x:c1.s -> my_reifiable (s2 x)) |}
   (wp:(x:c1.s -> st_wp (s2 x))) 
   : my_reifiable (x:c1.s -> STATEwp (s2 x) (wp x)) = {
-  s_tc = lang_effect_arrow c1.s #c1.s_tc s2 #(fun x -> (c2 x).s_tc) wp;
-  t = x:t1 -> mheap (c2 (c1.my_reflect x)).t (fun p -> wp (c1.my_reflect x) (fun (r:s2 (c1.my_reflect x)) -> p ((c2 (c1.my_reflect x)).my_reify r)));
+  s_tc = lang_effect_arrow c1.s #c1.s_tc s2 #(fun (x:c1.s) -> (c2 x).s_tc) wp;
+  t = x:t1 -> mheap (c2 (c1.my_reflect x)).t (fun (p:st_post (c2 (c1.my_reflect x)).t) -> wp (c1.my_reflect x) (fun (r:s2 (c1.my_reflect x)) -> p ((c2 (c1.my_reflect x)).my_reify r)));
   t_tc = lang_repr_arrow t1 #c1.t_tc (fun (x:t1) -> (c2 (c1.my_reflect x)).t) #(fun (x:t1) -> (c2 (c1.my_reflect x)).t_tc) _;
-  my_reify = (fun (f:(x:c1.s -> STATEwp (s2 x) (wp x))) ->
-    let f' (x:t1) : STATEwp (c2 (c1.my_reflect x)).t (fun p -> wp (c1.my_reflect x) (fun (r:s2 (c1.my_reflect x)) -> p ((c2 (c1.my_reflect x)).my_reify r))) = begin
-      let x' : c1.s = c1.my_reflect x in
-      let r : (s2 x') = f x' in
-      let r' : (c2 x').t = (c2 x').my_reify r in
-      admit ();
-      r'
-    end in
-    let f'' (x:t1) : mheap (c2 (c1.my_reflect x)).t (fun p -> wp (c1.my_reflect x) (fun (r:s2 (c1.my_reflect x)) -> p ((c2 (c1.my_reflect x)).my_reify r))) = begin
-      reify (f' x)
-    end in
-    f'');
+  my_reify = (fun (f:(x:c1.s -> STATEwp (s2 x) (wp x))) (x:t1) ->
+    reify (helper_reifiable_arrow' t1 #c1 s2 #c2 wp f x));
 }
 
 let fixed_wp #a : st_wp a =
   fun p h0 -> forall r h1. p r h1
+  
+let behT (f:(unit -> mheap int fixed_wp)) : st_wp int =
+  theta (f ())
+
+let behS (f:(unit -> STATEwp int fixed_wp)) : st_wp int =
+  theta (reify (f ()))
 
 let linkT
   (pt:((int -> mheap int fixed_wp) -> mheap int fixed_wp))
@@ -140,12 +182,6 @@ let linkS
   (unit -> STATEwp int fixed_wp)
   =
   fun () -> ps cs
-  
-let behT (f:(unit -> mheap int fixed_wp)) : st_wp int =
-  theta (f ())
-
-let behS (f:(unit -> STATEwp int fixed_wp)) : st_wp int =
-  theta (reify (f ()))
 
 val compile :
   ((int -> STATEwp int fixed_wp) -> STATEwp int fixed_wp) ->
@@ -172,20 +208,121 @@ type sc
   (ps:((int -> STATEwp int fixed_wp) -> STATEwp int fixed_wp))
   (ct:(int -> mheap int fixed_wp))
   =
-  behS (linkS ps (backtranslate ct)) == behT (linkT (compile ps) ct) (* syntactic equality between behaviors *)
+  behS (linkS ps (backtranslate ct)) `eq_wp` behT (linkT (compile ps) ct) (* syntactic equality between behaviors *)
 
-open FStar.Tactics.V2
+(** TODO: Why does this work? **)
+let reify_lemma (#a:Type) (#b:Type) (#wp:a -> st_wp b) (f:(x:a -> STATEwp b (wp x))) (x:a) : 
+  Lemma (
+    (theta (reify (let y = f x in y))) `eq_wp`
+    (theta (reify (f x)))) = ()
 
 let lemma_sc ps ct : Lemma (sc ps ct) by (
-  norm [delta_only [`%sc;`%behS;`%behT;`%compile;`%backtranslate;`%linkS;`%linkT;`%my_reflectable_arrow;`%my_reifiable_arrow;
-   `%lang_repr_arrow;`%lang_effect_arrow;`%my_reflectable_int;`%my_reifiable_int;`%lang_repr_int;`%lang_effect_int;
-   `%Mkmy_reflectable?.my_reflect;
-   `%Mkmy_reflectable?.s;
-   `%Mkmy_reifiable?.my_reify;
-   `%Mkmy_reifiable?.t;
-  ];zeta;delta;iota];
-  norm [iota];
- // tadmit (); (** looks the same, weird it fails, maybe because the previous admit? **)
-  dump "H"
+(**  norm [delta_only [
+                   `%sc;`%behS;`%behT;`%compile;`%backtranslate;`%linkS;`%linkT;
+                   `%my_reflectable_arrow;`%my_reifiable_arrow;
+                   `%lang_repr_arrow;`%lang_effect_arrow;`%my_reflectable_int;
+                   `%my_reifiable_int;`%lang_repr_int;`%lang_effect_int;
+                   `%Mkmy_reflectable?.my_reflect;`%Mkmy_reflectable?.s;
+                   `%Mkmy_reifiable?.my_reify;`%Mkmy_reifiable?.t;
+                   `%helper_reifiable_arrow';`%helper_reifiable_arrow;
+                   `%helper_reifiable_arrow_wp;
+       ];zeta;iota];**)
+  compute ()
 )= 
   ()
+
+(** ** The other setting **)
+
+let linkT'
+  (pt:(int -> mheap int fixed_wp))
+  (ct:((int -> mheap int fixed_wp) -> mheap int fixed_wp)) :
+  (unit -> mheap int fixed_wp)
+  =
+  fun () -> ct pt
+
+let linkS'
+  (ps:(int -> STATEwp int fixed_wp))
+  (cs:((int -> STATEwp int fixed_wp) -> STATEwp int fixed_wp)) :
+  (unit -> STATEwp int fixed_wp)
+  =
+  fun () -> cs ps
+
+val compile' :
+  (int -> STATEwp int fixed_wp) ->
+  (int -> mheap int fixed_wp)
+let compile' ps = 
+  (my_reifiable_arrow
+    int
+    #solve
+    (fun _ -> int) 
+    #(solve)
+    (fun _ -> fixed_wp)).my_reify ps
+
+val backtranslate' : 
+  ((int -> mheap int fixed_wp) -> mheap int fixed_wp) ->
+  ((int -> STATEwp int fixed_wp) -> STATEwp int fixed_wp)
+let backtranslate' ct =
+  (my_reflectable_arrow 
+    (int -> STATEwp int fixed_wp)
+    #(my_reifiable_arrow int #my_reflectable_int (fun _ -> int) #(fun _ -> my_reifiable_int) (fun _ -> fixed_wp))
+    (fun _ -> int) 
+    (fun _ -> fixed_wp)).my_reflect ct
+
+type sc'
+  (ps:(int -> STATEwp int fixed_wp))
+  (ct:((int -> mheap int fixed_wp) -> mheap int fixed_wp))
+  =
+  behS (linkS' ps (backtranslate' ct)) `eq_wp` behT (linkT' (compile' ps) ct) (* syntactic equality between behaviors *)
+
+let lemma_reify_reflect (f:mheap int 'w) :
+  Lemma (theta (reify (STATEwp?.reflect f)) `eq_wp` theta f) = admit ()
+
+let lemma_sc' ps ct : Lemma (sc' ps ct) = 
+  calc (eq_wp) {
+    behS (linkS' ps (backtranslate' ct));
+    `eq_wp` { 
+      _ by (
+        norm [delta_only [
+                    `%sc';`%behS;`%backtranslate';`%linkS';
+                    `%my_reflectable_arrow;`%my_reifiable_arrow;
+                    `%lang_repr_arrow;`%lang_effect_arrow;`%my_reflectable_int;
+                    `%my_reifiable_int;`%lang_repr_int;`%lang_effect_int;
+                    `%Mkmy_reflectable?.my_reflect;`%Mkmy_reflectable?.s;
+                    `%Mkmy_reifiable?.my_reify;`%Mkmy_reifiable?.t;
+                    `%helper_reifiable_arrow';`%helper_reifiable_arrow;
+                    `%helper_reifiable_arrow_wp;
+        ];zeta;iota]
+     )} 
+    theta (reify (STATEwp?.reflect (mheap_bind int int
+                            fixed_wp
+                            (fun r -> st_return heap_state.t int r)
+                            (ct (fun x -> reify (((let xxx = ps x in xxx)))))
+                            (fun r -> mheap_return int r))));
+    `eq_wp` { lemma_reify_reflect (mheap_bind int int
+                            fixed_wp
+                            (fun r -> st_return heap_state.t int r)
+                            (ct (fun x -> reify (((let xxx = ps x in xxx)))))
+                            (fun r -> mheap_return int r))}
+    theta (mheap_bind int int
+                            fixed_wp
+                            (fun r -> st_return heap_state.t int r)
+                            (ct (fun x -> reify (((let xxx = ps x in xxx)))))
+                            (fun r -> mheap_return int r));
+    `eq_wp` { 
+      lemma_theta_bind_id (ct (fun x -> reify (((let xxx = ps x in xxx))))) }
+    theta (ct (fun x -> reify (((let xxx = ps x in xxx)))));
+    `eq_wp` { 
+      _ by (
+        norm [delta_only [
+                    `%sc';`%behT;`%compile';`%linkT';
+                    `%my_reflectable_arrow;`%my_reifiable_arrow;
+                    `%lang_repr_arrow;`%lang_effect_arrow;`%my_reflectable_int;
+                    `%my_reifiable_int;`%lang_repr_int;`%lang_effect_int;
+                    `%Mkmy_reflectable?.my_reflect;`%Mkmy_reflectable?.s;
+                    `%Mkmy_reifiable?.my_reify;`%Mkmy_reifiable?.t;
+                    `%helper_reifiable_arrow';`%helper_reifiable_arrow;
+                    `%helper_reifiable_arrow_wp;
+        ];zeta;iota]
+     )} 
+    behT (linkT' (compile' ps) ct);
+  }
